CoqOfRust/core/default.v
@@ -1,0 +1,23 @@
+Require Import CoqOfRust.lib.lib.
+
+Module Impl_core_default_Default_for_u128.
+  Definition Self : Ty.t := Ty.path "u128".
+  
+  (*
+  fn default() -> $t {
+      $v
+  }
+  *)
+  Definition default (𝜏 : list Ty.t) (α : list Value.t) : M :=
+    match 𝜏, α with
+    | [], [] => M.pure (Value.Integer Integer.U128 0)
+    | _, _ => M.impossible
+    end.
+  
+  Axiom Implements :
+    M.IsTraitInstance
+      "core::default::Default"
+      (* Self *) (Ty.path "u128")
+      (* Trait polymorphic types *) []
+      (* Instance *) [ ("default", InstanceField.Method default) ].
+End Impl_core_default_Default_for_u128.
